Update coq backend library (WIP)

coq/Lib.v
@@ -5,435 +5,484 @@
 From Coq Require Import ZArith.
 (* Require Import Int.PArray. *)
 (* From Coq Require Import Numbers.Cyclic.Abstract.CyclicAxioms. *)
-From Coq Require Import Numbers.Cyclic.ZModulo.ZModulo.
+
+Require Import IntTypes.
 
 
-(**** Usize  *)
-(* TODO check this *)
-Definition U32 : N := 2^32 - 1.
-Definition S32 : Z := 2^31 - 1.
+Definition uint_size := N.
+(* Definition uint_size := range_t U32. *)
+Definition int_size := N.
+(* Definition int_size := range_t S32. *)
 
-Module uint32 : PositiveNotOne.
-  Definition p : positive := 2^32 - 1.
-  Theorem not_one : p <> 1%positive.
-  Proof. discriminate. Qed.    
-End uint32.
-
-Module U32 := ZModuloCyclicType uint32. Import U32.
-  
-
-(* 
-let uint_size = range_t U32
-let int_size = range_t S32 *)
 Open Scope N_scope.
-Definition uint_size := {n:N | n <= U32}.
-Open Scope Z_scope.
-Definition int_size := {n:Z | n <= S32}.
-
+Context {
+  uint_size_to_nat : uint_size -> nat
+}.
 (* Definition usize (n:range_t U32) : u:uint_size{u == n} := n *)
-Definition usize := uint_size.
-
 (* Definition isize (n:range_t S32) : u:int_size{u == n} := n *)
-Definition isize (n : {n : n < S32} : {u : u = n}:= int_size.
+Context {usize isize : N -> uint_size}.
+Context {
+  uint8
+  uint16
+  uint32
+  uint64
+  uint128
+  int8
+  int16
+  int32
+  int64
+  int128 
+  pub_uint8 
+  pub_int8 
+  pub_uint16 
+  pub_int16 
+  pub_uint32 
+  pub_int32 
+  pub_uint64 
+  pub_int64 
+  pub_uint128 
+  pub_int128 
+  : Type
+}.
+
+(* Definition size_t := uint_t U32 PUB *)
+(* Axiom uint_size : forall (n : inttype), n < U32. *)
+(* Axiom size : (n:size_nat) : size_t = uint #U32 #PUB n *)
+
+
 
 (**** Public integers *)
 
-Definition pub_u8 (n:range_t U8) : u:pub_uint8{v u == n} := uint #U8 #PUB n
+(* Definition pub_u8 (n:range_t U8) : u:pub_uint8{v u == n} := uint #U8 #PUB n *)
+Definition pub_u8 (n : range_t U8) := n.
 
-Definition pub_i8 (n:range_t S8) : u:pub_int8{v u == n} := sint #S8 #PUB n
+(* Definition pub_i8 (n:range_t S8) : u:pub_int8{v u == n} := sint #S8 #PUB n *)
+Definition pub_i8 (n : range_t S8) := n.
 
-Definition pub_u16 (n:range_t U16) : u:pub_uint16{v u == n} := uint #U16 #PUB n
+(* Definition pub_u16 (n:range_t U16) : u:pub_uint16{v u == n} := uint #U16 #PUB n *)
+Definition pub_u16 (n : range_t U16) := n.
 
-Definition pub_i16 (n:range_t S16) : u:pub_int16{v u == n} := sint #S16 #PUB n
+(* Definition pub_i16 (n:range_t S16) : u:pub_int16{v u == n} := sint #S16 #PUB n *)
+Definition pub_i16 (n : range_t S16) := n.
 
-Definition pub_u32 (n:range_t U32) : u:pub_uint32{v u == n} := uint #U32 #PUB n
+(* Definition pub_u32 (n:range_t U32) : u:pub_uint32{v u == n} := uint #U32 #PUB n *)
+Definition pub_u32 (n : range_t U32) := n.
 
-Definition pub_i32 (n:range_t S32) : u:pub_int32{v u == n} := sint #S32 #PUB n
+(* Definition pub_i32 (n:range_t S32) : u:pub_int32{v u == n} := sint #S32 #PUB n *)
+Definition pub_i32 (n : range_t S32) := n.
 
-Definition pub_u64 (n:range_t U64) : u:pub_uint64{v u == n} := uint #U64 #PUB n
+(* Definition pub_u64 (n:range_t U64) : u:pub_uint64{v u == n} := uint #U64 #PUB n *)
+Definition pub_u64 (n : range_t U64) := n.
 
-Definition pub_i64 (n:range_t S64) : u:pub_int64{v u == n} := sint #S64 #PUB n
+(* Definition pub_i64 (n:range_t S64) : u:pub_int64{v u == n} := sint #S64 #PUB n *)
+Definition pub_i64 (n : range_t S64) := n.
 
-Definition pub_u128 (n:range_t U128) : u:pub_uint128{v u == n} := uint #U128 #PUB n
+(* Definition pub_u128 (n:range_t U128) : u:pub_uint128{v u == n} := uint #U128 #PUB n *)
+Definition pub_u128 (n : range_t U128) := n.
 
-Definition pub_i128 (n:range_t S128) : u:pub_int128{v u == n} := sint #S128 #PUB n
+(* Definition pub_i128 (n:range_t S128) : u:pub_int128{v u == n} := sint #S128 #PUB n *)
+Definition pub_i128 (n : range_t S128) := n.
 
 (**** Operations *)
 
-Definition uint8_rotate_left (u: uint8) (s: uint_size{s > 0 /\ s < 8}) : uint8 =
-  rotate_left u (size s)
+Axiom size_t : Type.
+Axiom size : forall {intt : Type}, intt -> size_t.
+(* second argument is size *)
+Axiom rotate_left : forall {inttype : Type}, inttype -> size_t -> inttype.
+Axiom rotate_right : forall {inttype : Type}, inttype -> size_t -> inttype.
+Axiom shift_left : forall {inttype shiftval : Type}, inttype -> shiftval -> inttype.
+Axiom shift_right : forall {inttype shiftval : Type}, inttype -> shiftval -> inttype.
 
-Definition uint8_rotate_right (u: uint8) (s: uint_size{s > 0 /\ s < 8}) : uint8 =
-  rotate_right u (size s)
+Definition uint8_rotate_left (u: uint8) (s: uint8) : uint8 :=
+  rotate_left u (size s).
 
-Definition uint16_rotate_left (u: uint16) (s: uint_size{s > 0 /\ s < 16}) : uint16 =
-  rotate_left u (size s)
+Definition uint8_rotate_right (u: uint8) (s: uint8) : uint8 :=
+  rotate_right u (size s).
 
-Definition uint16_rotate_right (u: uint16) (s: uint_size{s > 0 /\ s < 16}) : uint16 =
-  rotate_right u (size s)
+Definition uint16_rotate_left (u: uint16) (s: uint16) : uint16 :=
+  rotate_left u (size s).
 
-Definition uint32_rotate_left (u: uint32) (s: uint_size{s > 0 /\ s < 32}) : uint32 =
-  rotate_left u (size s)
+Definition uint16_rotate_right (u: uint16) (s: uint16) : uint16 :=
+  rotate_right u (size s).
 
-Definition uint32_rotate_right (u: uint32) (s: uint_size{s > 0 /\ s < 32}) : uint32 =
-  rotate_right u (size s)
+Definition uint32_rotate_left (u: uint32) (s: uint32) : uint32 :=
+  rotate_left u (size s).
 
-Definition uint64_rotate_left (u: uint64) (s: uint_size{s > 0 /\ s < 64}) : uint64 =
-  rotate_left u (size s)
+Definition uint32_rotate_right (u: uint32) (s: uint32) : uint32 :=
+  rotate_right u (size s).
 
-Definition uint64_rotate_right (u: uint64) (s: uint_size{s > 0 /\ s < 64}) : uint64 =
-  rotate_right u (size s)
+Definition uint64_rotate_left (u: uint64) (s: uint64) : uint64 :=
+  rotate_left u (size s).
 
-Definition uint128_rotate_left (u: uint128) (s: uint_size{s > 0 /\ s < 128}) : uint128 =
-  rotate_left u (size s)
+Definition uint64_rotate_right (u: uint64) (s: uint64) : uint64 :=
+  rotate_right u (size s).
 
-Definition uint128_rotate_right (u: uint128) (s: uint_size{s > 0 /\ s < 128}) : uint128 =
-  rotate_right u (size s)
+Definition uint128_rotate_left (u: uint128) (s: uint128) : uint128 :=
+  rotate_left u (size s).
 
-Definition usize_shift_right (u: uint_size) (s: pub_uint32{v s < 32}) : uint_size =
-  v (shift_right (size u) s)
+Definition uint128_rotate_right (u: uint128) (s: uint128) : uint128 :=
+  rotate_right u (size s).
 
-Definition usize_shift_left (u: uint_size) (s: pub_uint32{v s < 32}) : uint_size =
-  v (shift_left (size u) s)
+Axiom to_uint_size : size_t -> uint_size.
 
-Definition pub_uint128_wrapping_add (x y: pub_uint128) : pub_uint128 =
-  x +. y
+Definition usize_shift_right (u: uint_size) (s: pub_uint32) : uint_size :=
+  to_uint_size (shift_right (size u) s).
+
+Definition usize_shift_left (u: uint_size) (s: pub_uint32) : uint_size :=
+  to_uint_size (shift_left (size u) s).
+
+
+Axiom pub_uint128_wrapping_add : pub_uint128 -> pub_uint128 -> pub_uint128. 
+  (* x +. y *)
 
 (*** Loops *)
 
-Definition rec foldi_
-  (#acc: Type)
-  (cur_i: uint_size)
-  (hi: uint_size{cur_i <:= hi})
-  (f: (i:uint_size{i < hi}) -> acc -> acc)
-  (cur: acc)
-    : Tot acc (decreases (hi - cur_i))
-  =
-  if cur_i := hi then cur else
-  foldi_ (cur_i + 1) hi f (f cur_i cur)
+Axiom foldi :
+  forall {acc: Type},
+  uint_size ->
+  uint_size ->
+  (uint_size -> acc -> acc) ->
+  acc -> acc.
 
-Definition foldi
-  (#acc: Type)
-  (lo: uint_size)
-  (hi: uint_size{lo <:= hi})
-  (f: (i:uint_size{i < hi}) -> acc -> acc)
-  (init: acc)
-    : acc
-  =
-  foldi_ lo hi f init
+(*** Sequences (lists) *)
+From Coq Require Import List.
 
-(*** Seq *)
+(* module LSeq := Lib.Sequence *)
+(* module LBSeq := Lib.ByteSequence *)
 
-module LSeq := Lib.Sequence
-module LBSeq := Lib.ByteSequence
+(* For now the size parameter is just discarded in the type... *)
+Inductive lseq (A : Type) (len : uint_size) : Type := 
+| mkLseq : list A -> lseq A len.
 
-Definition lseq (a: Type) (len: uint_size) := LSeq.lseq a len
+Definition lseq_to_list {A len} (s : lseq A len) := 
+  match s with
+  | mkLseq _ _ l => l
+  end.
 
-Definition seq (a: Type) := s:LSeq.seq a{range (LSeq.length s) U32}
- Definition byte_seq := seq uint8
+(* simplification *)
+Definition seq (A : Type) := list A.
 
-Definition nseq (a: Type) (len: nat) := s:LSeq.seq a{LSeq.length s == len}
+Definition byte_seq := seq uint8.
 
-Definition seq_len (#a: Type) (s: seq a) : nat := Seq.length s
+Definition nseq (A : Type) (len: nat) := list A.
 
-Definition seq_new_ (#a: Type) (init:a) (len: uint_size) : lseq a len =
-  Seq.create len init
+Definition seq_len {A: Type} (s: seq A) : nat := List.length s.
 
-Definition array_from_list
-  (#a: Type)
-  (l: list a{List.Tot.length l <:= max_size_t})
-    : lseq a (List.Tot.length l)
-  =
-  LSeq.of_list l
+Definition seq_new_ {A: Type} (init : A) (len: uint_size) : lseq A len :=
+  mkLseq _ _ (List.repeat init (N.to_nat len)).
+
+Definition array_from_list {A: Type} (l: list A) : lseq A (N.of_nat (List.length l))
+  := mkLseq _ (N.of_nat (List.length l)) l.
 
 (**** Array manipulation *)
 
 
-Definition array_new_ (#a: Type) (init:a) (len: uint_size)  : lseq a len =
-  LSeq.create len init
+Definition array_new_ {A: Type} (init:A) (len: uint_size)  : lseq A len :=
+  mkLseq _ _ (List.repeat init (N.to_nat len)).
+  
+(* Definition array_index {A: Type} {len : uint_size} (s: lseq A len) (i: uint_size) : A :=
+  List.nth (N.to_nat i) (lseq_to_list s). *)
 
-Definition array_index (#a: Type) (#len:uint_size) (s: lseq a len) (i: uint_size{i < len}) : a =
-  LSeq.index s i
-
-Definition array_upd (#a: Type) (#len:uint_size) (s: lseq a len) (i: uint_size{i < len}) (new_v: a) : lseq a len := LSeq.upd s i new_v
+(* Definition array_upd {A: Type} {len : uint_size} (s: lseq A len) (i: uint_size) (new_v: A) : lseq A len := List.upd s i new_v.
 
 Definition array_from_seq
-  (#a: Type)
+  {A: Type}
   (out_len:uint_size)
-  (input: seq a{Seq.length input := out_len})
-    : lseq a out_len
-  := input
+  (input: seq a{Seq.length input ::= out_len})
+    : lseq A out_len
+  := input.
 
 Definition array_from_slice
-  (#a: Type)
+  {A: Type}
   (default_value: a)
   (out_len: uint_size)
   (input: seq a)
   (start: uint_size)
-  (slice_len: uint_size{start + slice_len <:= LSeq.length input /\ slice_len <:= out_len})
-    : lseq a out_len
-  =
-  Definition out := LSeq.create out_len default_value in
-  LSeq.update_sub out 0 slice_len (LSeq.slice #a #(Seq.length input) input start (start + slice_len))
+  (slice_len: uint_size{start + slice_len <::= LSeq.length input /\ slice_len <::= out_len})
+    : lseq A out_len
+  :=
+  let out ::= LSeq.create out_len default_value in
+  LSeq.update_sub out 0 slice_len (LSeq.slice #a #(Seq.length input) input start (start + slice_len)).
 
 Definition array_slice
-  (#a: Type)
+  {A: Type}
   (input: seq a)
   (start: uint_size)
-  (slice_len: uint_size{start + slice_len <:= LSeq.length input})
-    : lseq a slice_len
-  =
-  Seq.slice input start (start + slice_len)
+  (slice_len: uint_size{start + slice_len <::= LSeq.length input})
+    : lseq A slice_len
+  :=
+  Seq.slice input start (start + slice_len).
 
 Definition array_from_slice_range
-  (#a: Type)
+  {A: Type}
   (default_value: a)
   (out_len: uint_size)
   (input: seq a)
   (start_fin: (uint_size & uint_size){
-     fst start_fin >:= 0 /\ snd start_fin <:= LSeq.length input /\ snd start_fin >:= fst start_fin /\
-     snd start_fin - fst start_fin <:= out_len
+     fst start_fin >::= 0 /\ snd start_fin <::= LSeq.length input /\ snd start_fin >::= fst start_fin /\
+     snd start_fin - fst start_fin <::= out_len
    })
-    : lseq a out_len
-  =
-  Definition out := array_new_ default_value out_len in
-  Definition (start, fin) := start_fin in
-  LSeq.update_sub out 0 (fin - start) (Seq.slice input start fin)
+    : lseq A out_len
+ :=
+  let out ::= array_new_ default_value out_len in
+  let (start, fin) ::= start_fin in
+  LSeq.update_sub out 0 (fin - start) (Seq.slice input start fin).
 
 Definition array_slice_range
-  (#a: Type)
-  (#len:uint_size)
-  (input: lseq a len)
+  {A: Type}
+  {len : uint_size}
+  (input: lseq A len)
   (start_fin:(uint_size & uint_size){
-    fst start_fin >:= 0 /\ snd start_fin <:= len /\ snd start_fin >:= fst start_fin
+    fst start_fin >::= 0 /\ snd start_fin <::= len /\ snd start_fin >::= fst start_fin
   })
-    : lseq a (snd start_fin - fst start_fin)
-  =
-  Definition (start, fin) := start_fin in
-  LSeq.slice input start fin
+    : lseq A (snd start_fin - fst start_fin)uint_size
+  :=
+  let (start, fin) ::= start_fin in
+  LSeq.slice input start fin.
 
 Definition array_update_start
-  (#a: Type)
+  {A: Type}
   (#len: uint_size)
-  (s: lseq a len)
-  (start_s: seq a{Seq.length start_s <:= len})
-    : lseq a len
-  =
-  LSeq.update_sub s 0 (Seq.length start_s) start_s
+  (s: lseq A len)
+  (start_s: seq a{Seq.length start_s <::= len})
+    : lseq A len
+  :=
+  LSeq.update_sub s 0 (Seq.length start_s) start_s.
 
-Definition array_len  (#a: Type) (#len: uint_size) (s: lseq a len) := len
+Definition array_len  {A: Type} (#len: uint_size) (s: lseq A len) := len
 
-(**** Seq manipulation *)
+(**** Seq manipulation *).
 
 Definition seq_slice
-  (#a: Type)
+  {A: Type}
   (s: seq a)
   (start: uint_size)
-  (len: uint_size{start + len <:= LSeq.length s})
-    : lseq a len
-  =
-  LSeq.slice #a #(Seq.length s) s start (start + len)
+  (len: uint_size{start + len <::= LSeq.length s})
+    : lseq A len
+  :=
+  LSeq.slice #a #(Seq.length s) s start (start + len).
 
 Definition seq_update
-  (#a: Type)
+  {A: Type}
   (s: seq a)
   (start: uint_size)
-  (input: seq a{start + LSeq.length input <:= LSeq.length s})
+  (input: seq a{start + LSeq.length input <::= LSeq.length s})
     : nseq a (LSeq.length s)
-  =
-  LSeq.update_sub #a #(LSeq.length s) s start (LSeq.length input) input
+  :=
+  LSeq.update_sub #a #(LSeq.length s) s start (LSeq.length input) input.
 
 Definition seq_concat
-  (#a: Type)
+  {A: Type}
   (s1 :seq a)
   (s2: seq a{range (LSeq.length s1 + LSeq.length s2) U32})
-  : lseq a (LSeq.length s1 + LSeq.length s2)
-  =
+  : lseq A (LSeq.length s1 + LSeq.length s2)
+  :=
   LSeq.concat #a #(LSeq.length s1) #(LSeq.length s2) s1 s2
 
 
-(**** Chunking *)
+(**** Chunking *).
 
-Definition seq_num_chunks (#a: Type) (s: seq a) (chunk_len: uint_size{chunk_len > 0}) : uint_size =
-  (Seq.length s + chunk_len - 1) / chunk_len
+Definition seq_num_chunks {A: Type} (s: seq a) (chunk_len: uint_size{chunk_len > 0}) : uint_size :=
+  (Seq.length s + chunk_len - 1) / chunk_len.
 
 Definition seq_chunk_len
-  (#a: Type)
+  {A: Type}
   (s: seq a)
   (chunk_len: uint_size)
-  (chunk_num: uint_size{chunk_len * chunk_num <:= Seq.length s})
-    : Tot (out_len:uint_size{out_len <:= chunk_len})
-  =
-  Definition idx_start := chunk_len * chunk_num in
+  (chunk_num: uint_size{chunk_len * chunk_num <::= Seq.length s})
+    : Tot (out_len:uint_size{out_len <::= chunk_len})
+ . :=
+  Definition idx_start ::= chunk_len * chunk_num in
   if idx_start + chunk_len > Seq.length s then
     Seq.length s - idx_start
   else
-    chunk_len
+    chunk_len.
 
 Definition seq_chunk_same_len_same_chunk_len
-  (#a: Type)
+  {A: Type}
   (s1 s2: seq a)
   (chunk_len: uint_size)
   (chunk_num: uint_size)
   : Lemma
-    (requires (LSeq.length s1 := LSeq.length s2 /\ chunk_len * chunk_num <:= Seq.length s1))
-    (ensures (seq_chunk_len s1 chunk_len chunk_num := seq_chunk_len s2 chunk_len chunk_num))
-    [SMTPat (seq_chunk_len s1 chunk_len chunk_num); SMTPat (seq_chunk_len s2 chunk_len chunk_num)]
-  =
-  ()
+    (requires (LSeq.length s1 ::= LSeq.length s2 /\ chunk_len * chunk_num <::= Seq.length s1))
+    (ensures (seq_chunk_len s1 chunk_len chunk_lseq.
 
 Definition seq_get_chunk
-  (#a: Type)
+  {A: Type}
   (s: seq a)
   (chunk_len: uint_size)
   (chunk_num: uint_size)
   : Pure (uint_size & seq a)
-    (requires (chunk_len * chunk_num <:= Seq.length s))
+    (requires (chunk_len * chunk_num <::= Seq.length s))
     (ensures (fun (out_len, chunk) ->
-      out_len := seq_chunk_len s chunk_len chunk_num /\ LSeq.length chunk := out_len
+      out_len ::= seq_chunk_len s chunk_len chunk_num /\ LSeq.length chunk ::= out_len
     ))
-  =
-  Definition idx_start := chunk_len * chunk_num in
-  Definition out_len := seq_chunk_len s chunk_len chunk_num in
+ . :=
+  Definition idx_start ::= chunk_len * chunk_num in
+  Definition out_len ::= seq_chunk_len s chunk_len chunk_num in
   (out_len, LSeq.slice #a #(Seq.length s)
     s idx_start (idx_start + seq_chunk_len s chunk_len chunk_num))
 
 Definition seq_set_chunk
-  (#a: Type)
-  (#len:uint_size) (* change to nseq but update_sub missing for nseq *)
-  (s: lseq a len)
+  {A: Type}
+  {len : uint_size} (* change to nseq but update_sub missing for nseq *)
+  (s: lseq A len)
   (chunk_len: uint_size)
   (chunk_num: uint_size)
   (chunk: seq a )
-    : Pure (lseq a len)
+    : Pure (lseq A len)
       (requires (
-        chunk_len * chunk_num <:= Seq.length s /\
-        LSeq.length chunk := seq_chunk_len s chunk_len chunk_num
+        chunk_len * chunk_num <::= Seq.length s /\
+        LSeq.length chunk ::= seq_chunk_len s chunk_len chunk_num
       ))
       (ensures (fun out -> True))
-  =
-  Definition idx_start := chunk_len * chunk_num in
-  Definition out_len := seq_chunk_len s chunk_len chunk_num in
+  :=
+  Definition idx_start ::= chunk_len * chunk_num in
+  Definition out_len ::= seq_chunk_len s chunk_len chunk_num in
   LSeq.update_sub s idx_start out_len chunk
 
 (**** Numeric operations *)
 
 Definition array_xor
-  (#a: Type)
+  {A: Type}
   (#len: uint_size)
   (xor: a -> a -> a)
-  (s1: lseq a len)
-  (s2 : lseq a len)
-    : lseq a len
-  =
-  Definition out := s1 in
+  (s1: lseq A len)
+  (s2 : lseq A len)
+    : lseq A len
+  :=
+  Definition out ::= s1 in
   foldi 0 len (fun i out ->
     array_upd out i (array_index s1 i `xor` array_index s2 i)
   ) out
 
 Definition array_eq
-  (#a: Type)
+  {A: Type}
   (#len: uint_size)
   (eq: a -> a -> bool)
-  (s1: lseq a len)
-  (s2 : lseq a len)
+  (s1: lseq A len)
+  (s2 : lseq A len)
     : bool
-  =
-  Definition out := true in
+  :=
+  Definition out ::= true in
   foldi 0 len (fun i out ->
     out && (array_index s1 i `eq` array_index s2 i)
-  ) out
+  ) out *)
 
 (**** Integers to arrays *)
+(* 
+Definition uint32_to_le_bytes (x: uint32) : lseq uint8 4 :=
+  LBSeq.uint_to_bytes_le x.
 
-Definition uint32_to_le_bytes (x: uint32) : lseq uint8 4 =
-  LBSeq.uint_to_bytes_le x
-
-Definition uint32_to_be_bytes (x: uint32) : lseq uint8 4 =
+Definition uint32_to_be_bytes (x: uint32) : lseq uint8 4 :=
   LBSeq.uint_to_bytes_be x
 
-Definition uint32_from_le_bytes (s: lseq uint8 4) : uint32 =
+Definition uint32_from_le_bytes (s: lseq uint8 4) : uint32 :=
   LBSeq.uint_from_bytes_le s
 
-Definition uint32_from_be_bytes (s: lseq uint8 4) : uint32 =
+Definition uint32_from_be_bytes (s: lseq uint8 4) : uint32 :=
   LBSeq.uint_from_bytes_be s
 
-Definition uint64_to_le_bytes (x: uint64) : lseq uint8 8 =
+Definition uint64_to_le_bytes (x: uint64) : lseq uint8 8 :=
   LBSeq.uint_to_bytes_le x
 
-Definition uint64_to_be_bytes (x: uint64) : lseq uint8 8 =
+Definition uint64_to_be_bytes (x: uint64) : lseq uint8 8 :=
   LBSeq.uint_to_bytes_be x
 
-Definition uint64_from_le_bytes (s: lseq uint8 8) : uint64 =
+Definition uint64_from_le_bytes (s: lseq uint8 8) : uint64 :=
   LBSeq.uint_from_bytes_le s
 
-Definition uint64_from_be_bytes (s: lseq uint8 8) : uint64 =
+Definition uint64_from_be_bytes (s: lseq uint8 8) : uint64 :=
   LBSeq.uint_from_bytes_be s
 
-Definition uint128_to_le_bytes (x: uint128) : lseq uint8 16 =
+Definition uint128_to_le_bytes (x: uint128) : lseq uint8 16 :=
   LBSeq.uint_to_bytes_le x
 
-Definition uint128_to_be_bytes (x: uint128) : lseq uint8 16 =
+Definition uint128_to_be_bytes (x: uint128) : lseq uint8 16 :=
   LBSeq.uint_to_bytes_be x
 
-Definition uint128_from_le_bytes (input: lseq uint8 16) : uint128 =
+Definition uint128_from_le_bytes (input: lseq uint8 16) : uint128 :=
   LBSeq.uint_from_bytes_le input
 
-Definition uint128_from_be_bytes (s: lseq uint8 16) : uint128 =
+Definition uint128_from_be_bytes (s: lseq uint8 16) : uint128 :=
   LBSeq.uint_from_bytes_be s
 
-Definition u32_to_le_bytes (x: pub_uint32) : lseq pub_uint8 4 =
+Definition u32_to_le_bytes (x: pub_uint32) : lseq pub_uint8 4 :=
   LBSeq.uint_to_bytes_le x
 
-Definition u32_to_be_bytes (x: pub_uint32) : lseq pub_uint8 4 =
+Definition u32_to_be_bytes (x: pub_uint32) : lseq pub_uint8 4 :=
   LBSeq.uint_to_bytes_be x
 
-Definition u32_from_le_bytes (s: lseq pub_uint8 4) : pub_uint32 =
+Definition u32_from_le_bytes (s: lseq pub_uint8 4) : pub_uint32 :=
   LBSeq.uint_from_bytes_le s
 
-Definition u32_from_be_bytes (s: lseq pub_uint8 4) : pub_uint32 =
+Definition u32_from_be_bytes (s: lseq pub_uint8 4) : pub_uint32 :=
   LBSeq.uint_from_bytes_be s
 
-Definition u64_to_le_bytes (x: pub_uint64) : lseq pub_uint8 8 =
+Definition u64_to_le_bytes (x: pub_uint64) : lseq pub_uint8 8 :=
   LBSeq.uint_to_bytes_le x
 
-Definition u64_to_be_bytes (x: pub_uint64) : lseq pub_uint8 8 =
+Definition u64_to_be_bytes (x: pub_uint64) : lseq pub_uint8 8 :=
   LBSeq.uint_to_bytes_be x
 
-Definition u64_from_le_bytes (s: lseq pub_uint8 8) : pub_uint64 =
+Definition u64_from_le_bytes (s: lseq pub_uint8 8) : pub_uint64 :=
   LBSeq.uint_from_bytes_le s
 
-Definition u64_from_be_bytes (s: lseq pub_uint8 8) : pub_uint64 =
+Definition u64_from_be_bytes (s: lseq pub_uint8 8) : pub_uint64 :=
   LBSeq.uint_from_bytes_be s
 
-Definition u128_to_le_bytes (x: pub_uint128) : lseq pub_uint8 16 =
+Definition u128_to_le_bytes (x: pub_uint128) : lseq pub_uint8 16 :=
   LBSeq.uint_to_bytes_le x
 
-Definition u128_to_be_bytes (x: pub_uint128) : lseq pub_uint8 16 =
+Definition u128_to_be_bytes (x: pub_uint128) : lseq pub_uint8 16 :=
   LBSeq.uint_to_bytes_be x
 
-Definition u128_from_le_bytes (input: lseq pub_uint8 16) : pub_uint128 =
+Definition u128_from_le_bytes (input: lseq pub_uint8 16) : pub_uint128 :=
   LBSeq.uint_from_bytes_le input
 
-Definition u128_from_be_bytes (s: lseq pub_uint8 16) : pub_uint128 =
-  LBSeq.uint_from_bytes_be s
+Definition u128_from_be_bytes (s: lseq pub_uint8 16) : pub_uint128 :=
+  LBSeq.uint_from_bytes_be s *)
 
 (*** Nats *)
+Close Scope N_scope.
 
-Definition nat_mod (n: nat) := x:nat{x < n}
+(* type representing nats less than n *)
+Definition nat_mod (n: nat) := nat.
+(* Definition nat_mod (n: nat) := {x : nat | x < n}. *)
 
-val (+%) (#n:pos) (a:nat_mod n) (b:nat_mod n) : nat_mod n
-Definition (+%) #n a b := (a + b) % n
+(* 
+Definition nat_mod_add {n:nat} (a:nat_mod n) (b:nat_mod n) : nat_mod n.
+Proof.
+  unfold nat_mod. destruct a. destruct b.
+  apply (exist _ (x + x0 mod n)).
+   *)
+Definition nat_mod_add {n:nat} (a:nat_mod n) (b:nat_mod n) : nat_mod n :=
+   (a + b) mod n.
 
-val ( *% ) (#n:pos) (a:nat_mod n) (b:nat_mod n) : nat_mod n
-Definition ( *% ) #n a b := (a * b) % n
+Notation "a + b" :=
+  (nat_mod_add)
+  : hacspec_scope.
 
-Definition nat_from_secret_literal (m:pos) (x:uint128{v x < m}) : n:nat_mod m{v x == n} =
-  v x
 
-Definition nat_from_literal (m: pos) (x:pub_uint128{v x < m}) : n:nat_mod m{v x == n} =
-  v x
+Definition nat_mod_mul {n:nat} (a:nat_mod n) (b:nat_mod n) : nat_mod n :=
+  (a * b) mod n.
 
+Notation "a * b" :=
+  (nat_mod_mul)
+  : hacspec_scope.
+
+
+Axiom uint128_to_nat : uint128 -> nat.
+
+Definition nat_from_secret_literal (m:nat) (x:uint128) : nat_mod m :=
+  uint128_to_nat x.
+
+Axiom pub_uint128_to_nat : pub_uint128 -> nat.
+
+Definition nat_from_literal (m:nat) (x:pub_uint128) : nat_mod m :=
+  pub_uint128_to_nat x.
+
+  
 Definition nat_to_public_byte_seq_le (n: pos)  (len: uint_size) (x: nat_mod n) : lseq pub_uint8 len =
   Definition n' := n % (pow2 (8 * len)) in
   Lib.ByteSequence.nat_to_bytes_le len n'
